src/program_proof/tulip/msg.v
@@ -22,13 +22,51 @@ Instance txnreq_countable :
   Countable txnreq.
 Admitted.
 
-Definition encode_fast_prepare_req (ts : u64) (pwrs : dbmap) (data : list u8) :=
-  ∃ datapwrs, data = u64_le (U64 201) ++ u64_le ts ++ datapwrs ∧ encode_dbmap pwrs datapwrs.
+Definition encode_read_req_xkind (ts : u64) (key : string) :=
+  u64_le ts ++ encode_string key.
+
+Definition encode_read_req (ts : u64) (key : string) (data : list u8) :=
+  data = u64_le (U64 100) ++ encode_read_req_xkind ts key.
+
+Definition encode_fast_prepare_req_xkind (ts : u64) (m : dbmap) (data : list u8) :=
+  ∃ mdata, data = u64_le ts ++ mdata ∧ encode_dbmap m mdata.
+
+Definition encode_fast_prepare_req (ts : u64) (m : dbmap) (data : list u8) :=
+  ∃ reqdata, data = u64_le (U64 201) ++ reqdata ∧ encode_fast_prepare_req_xkind ts m reqdata.
+
+Definition encode_validate_req_xkind (ts rank : u64) (m : dbmap) (data : list u8) :=
+  ∃ mdata, data = u64_le ts ++ u64_le rank ++ mdata ∧ encode_dbmap m mdata.
+
+Definition encode_validate_req (ts rank : u64) (m : dbmap) (data : list u8) :=
+  ∃ reqdata, data = u64_le (U64 202) ++ reqdata ∧ encode_validate_req_xkind ts rank m reqdata.
+
+Definition encode_req_of_ts_rank_xkind (ts rank : u64) := u64_le ts ++ u64_le rank.
+
+Definition encode_req_of_ts_rank (kind : u64) (ts rank : u64) (data : list u8) :=
+  data = u64_le kind ++ encode_req_of_ts_rank_xkind ts rank.
+
+Definition encode_commit_req_xkind (ts : u64) (m : dbmap) (data : list u8) :=
+  ∃ mdata, data = u64_le ts ++ mdata ∧ encode_dbmap m mdata.
+
+Definition encode_commit_req (ts : u64) (m : dbmap) (data : list u8) :=
+  ∃ reqdata, data = u64_le (U64 300) ++ reqdata ∧ encode_commit_req_xkind ts m reqdata.
+
+Definition encode_abort_req_xkind (ts : u64) := u64_le ts.
+
+Definition encode_abort_req (ts : u64) (data : list u8) :=
+  data = u64_le (U64 301) ++ encode_abort_req_xkind ts.
 
 Definition encode_txnreq (req : txnreq) (data : list u8) :=
   match req with
+  | ReadReq ts key => encode_read_req ts key data
   | FastPrepareReq ts pwrs => encode_fast_prepare_req ts pwrs data
-  | _ => True
+  | ValidateReq ts rank pwrs => encode_validate_req ts rank pwrs data
+  | PrepareReq ts rank => encode_req_of_ts_rank (U64 203) ts rank data
+  | UnprepareReq ts rank => encode_req_of_ts_rank (U64 204) ts rank data
+  | QueryReq ts rank => encode_req_of_ts_rank (U64 205) ts rank data
+  | RefreshReq ts rank => encode_req_of_ts_rank (U64 210) ts rank data
+  | CommitReq ts pwrs => encode_commit_req ts pwrs data
+  | AbortReq ts => encode_abort_req ts data
   end.
 
 Inductive rpres :=
@@ -41,7 +79,7 @@ Inductive rpres :=
 | ReplicaWrongLeader.
 
 #[global]
-  Instance rpres_eq_decision :
+Instance rpres_eq_decision :
   EqDecision rpres.
 Proof. solve_decision. Qed.
 
@@ -56,12 +94,12 @@ Inductive txnresp :=
 | AbortResp       (ts : u64) (res : rpres).
 
 #[global]
-  Instance txnresp_eq_decision :
+Instance txnresp_eq_decision :
   EqDecision txnresp.
 Proof. solve_decision. Qed.
 
 #[global]
-  Instance txnresp_countable :
+Instance txnresp_countable :
   Countable txnresp.
 Admitted.
 
