src/program_proof/tulip/program/gcoord/gcoord_send.v
@@ -1,21 +1,6 @@
 From Perennial.program_proof.tulip.program Require Import prelude.
 From Perennial.program_proof.tulip.program.gcoord Require Import
-  gcoord_repr gcoord_get_connection gcoord_connect.
-
-Section encode.
-  Context `{!heapGS Σ, !paxos_ghostG Σ}.
-
-  Theorem wp_EncodeTxnReadRequest (ts : u64) (key : string) :
-    {{{ True }}}
-      EncodeTxnReadRequest #ts #(LitString key)
-    {{{ (dataP : Slice.t) (data : list u8), RET (to_val dataP);
-        own_slice dataP byteT (DfracOwn 1) data ∗
-        ⌜encode_txnreq (ReadReq ts key) data⌝
-    }}}.
-  Proof.
-  Admitted.
-
-End encode.
+  gcoord_repr gcoord_get_connection gcoord_connect encode.
 
 Section program.
   Context `{!heapGS Σ, !tulip_ghostG Σ}.
@@ -167,99 +152,642 @@ Section program.
   Qed.
 
   Theorem wp_GroupCoordinator__SendFastPrepare
-    (gcoord : loc) (rid : u64) (ts : u64) (pwrsP : loc) (ptgsP : Slice.t) gid γ :
-    is_gcoord gcoord gid γ -∗
-    {{{ True }}}
-      GroupCoordinator__SendFastPrepare #gcoord #rid #ts #pwrsP (to_val ptgsP)
+    (gcoord : loc) (rid : u64) (tsW : u64) (pwrsP : loc) (ptgsP : Slice.t) q (pwrs : dbmap)
+    addrm gid γ :
+    let ts := uint.nat tsW in
+    rid ∈ dom addrm ->
+    safe_txn_pwrs γ gid ts pwrs -∗
+    is_gcoord_with_addrm gcoord gid addrm γ -∗
+    {{{ own_map pwrsP q pwrs }}}
+      GroupCoordinator__SendFastPrepare #gcoord #rid #tsW #pwrsP (to_val ptgsP)
     {{{ RET #(); True }}}.
   Proof.
+    iIntros (ts Hrid) "#Hsafepwrs #Hgcoord".
+    iIntros (Φ) "!> Hpwrs HΦ".
+    wp_rec.
+
     (*@ func (gcoord *GroupCoordinator) SendFastPrepare(rid, ts uint64, pwrs tulip.KVMap, ptgs []uint64) { @*)
     (*@     gcoord.Send(rid, message.EncodeTxnFastPrepare(ts, pwrs, ptgs))      @*)
     (*@ }                                                                       @*)
-  Admitted.
+    wp_apply (wp_EncodeTxnFastPrepareRequest with "Hpwrs").
+    iIntros (dataP data) "(Hdata & Hpwrs & %Hdataenc)".
+    iNamed "Hgcoord".
+    iNamed "Haddrm".
+    assert (is_Some (addrm !! rid)) as [addrpeer Haddrpeer].
+    { by apply elem_of_dom. }
+    wp_apply (wp_GroupCoordinator__Send with "[] Hdata"); first apply Haddrpeer.
+    { iFrame "# %". }
+    iInv "Hinvnet" as "> HinvnetO" "HinvnetC".
+    iApply ncfupd_mask_intro; first set_solver.
+    iIntros "Hmask".
+    iNamed "HinvnetO".
+    assert (is_Some (listens !! addrpeer)) as [ms Hms].
+    { rewrite -elem_of_dom -Himgaddrm elem_of_map_img. by eauto. }
+    iDestruct (big_sepM_delete with "Hlistens") as "[Hlst Hlistens]"; first apply Hms.
+    iNamed "Hlst".
+    iFrame "Hms".
+    iIntros (sent) "Hms".
+    destruct sent; last first.
+    { iDestruct (big_sepM_insert_2 _ _ addrpeer ms with "[Hms] Hlistens") as "Hlistens".
+      { iFrame "∗ # %". }
+      rewrite insert_delete; last apply Hms.
+      iMod "Hmask" as "_".
+      iMod ("HinvnetC" with "[$Hlistens $Hconnects $Hterminals]") as "_".
+      { done. }
+      iIntros "!> _".
+      wp_pures.
+      by iApply "HΦ".
+    }
+    iDestruct "Hms" as (trml) "[Hms #Htrml]".
+    set ms' := _ ∪ ms.
+    iDestruct (big_sepM_insert_2 _ _ addrpeer ms' with "[Hms] Hlistens") as "Hlistens".
+    { iFrame "Hms".
+      set req := FastPrepareReq _ _ in Hdataenc.
+      iExists ({[req]} ∪ reqs).
+      iSplit.
+      { rewrite set_map_union_L set_map_singleton_L.
+        by iApply big_sepS_insert_2.
+      }
+      iSplit.
+      { iApply big_sepS_insert_2; [done | done]. }
+      iPureIntro.
+      apply set_Forall_union; last first.
+      { apply (set_Forall_impl _ _ _ Henc). intros m Hm. clear -Hm. set_solver. }
+      rewrite set_Forall_singleton.
+      exists req.
+      split; first set_solver.
+      done.
+    }
+    rewrite insert_delete_insert.
+    iMod "Hmask" as "_".
+    iMod ("HinvnetC" with "[$Hlistens $Hconnects $Hterminals]") as "_".
+    { iPureIntro.
+      rewrite dom_insert_L Himgaddrm.
+      apply (elem_of_map_img_2 (SA := gset chan)) in Haddrpeer.
+      set_solver.
+    }
+    iIntros "!> _".
+    wp_pures.
+    by iApply "HΦ".
+  Qed.
 
   Theorem wp_GroupCoordinator__SendValidate
-    (gcoord : loc) (rid : u64) (ts : u64) (rank : u64) (pwrsP : loc) (ptgsP : Slice.t) gid γ :
-    is_gcoord gcoord gid γ -∗
-    {{{ True }}}
-      GroupCoordinator__SendValidate #gcoord #rid #ts #rank #pwrsP (to_val ptgsP)
+    (gcoord : loc) (rid : u64) (tsW : u64) (pwrsP : loc) (ptgsP : Slice.t)
+    q (pwrs : dbmap) addrm gid γ :
+    let ts := uint.nat tsW in
+    rid ∈ dom addrm ->
+    safe_txn_pwrs γ gid ts pwrs -∗
+    is_gcoord_with_addrm gcoord gid addrm γ -∗
+    {{{ own_map pwrsP q pwrs }}}
+      GroupCoordinator__SendValidate #gcoord #rid #tsW #pwrsP (to_val ptgsP)
     {{{ RET #(); True }}}.
   Proof.
-    (*@ func (gcoord *GroupCoordinator) SendValidate(rid, ts, rank uint64, pwrs tulip.KVMap, ptgs []uint64) { @*)
+    iIntros (ts Hrid) "#Hsafepwrs #Hgcoord".
+    iIntros (Φ) "!> Hpwrs HΦ".
+    wp_rec.
+
+    (*@ func (gcoord *GroupCoordinator) SendValidate(rid, ts uint64, pwrs tulip.KVMap, ptgs []uint64) { @*)
+    (*@     data := message.EncodeTxnValidateRequest(ts, 1, pwrs, ptgs)         @*)
+    (*@     gcoord.Send(rid, data)                                              @*)
     (*@ }                                                                       @*)
-  Admitted.
+    wp_apply (wp_EncodeTxnValidateRequest with "Hpwrs").
+    iIntros (dataP data) "(Hdata & Hpwrs & %Hdataenc)".
+    iNamed "Hgcoord".
+    iNamed "Haddrm".
+    assert (is_Some (addrm !! rid)) as [addrpeer Haddrpeer].
+    { by apply elem_of_dom. }
+    wp_apply (wp_GroupCoordinator__Send with "[] Hdata"); first apply Haddrpeer.
+    { iFrame "# %". }
+    iInv "Hinvnet" as "> HinvnetO" "HinvnetC".
+    iApply ncfupd_mask_intro; first set_solver.
+    iIntros "Hmask".
+    iNamed "HinvnetO".
+    assert (is_Some (listens !! addrpeer)) as [ms Hms].
+    { rewrite -elem_of_dom -Himgaddrm elem_of_map_img. by eauto. }
+    iDestruct (big_sepM_delete with "Hlistens") as "[Hlst Hlistens]"; first apply Hms.
+    iNamed "Hlst".
+    iFrame "Hms".
+    iIntros (sent) "Hms".
+    destruct sent; last first.
+    { iDestruct (big_sepM_insert_2 _ _ addrpeer ms with "[Hms] Hlistens") as "Hlistens".
+      { iFrame "∗ # %". }
+      rewrite insert_delete; last apply Hms.
+      iMod "Hmask" as "_".
+      iMod ("HinvnetC" with "[$Hlistens $Hconnects $Hterminals]") as "_".
+      { done. }
+      iIntros "!> _".
+      wp_pures.
+      by iApply "HΦ".
+    }
+    iDestruct "Hms" as (trml) "[Hms #Htrml]".
+    set ms' := _ ∪ ms.
+    iDestruct (big_sepM_insert_2 _ _ addrpeer ms' with "[Hms] Hlistens") as "Hlistens".
+    { iFrame "Hms".
+      set req := ValidateReq _ _ _ in Hdataenc.
+      iExists ({[req]} ∪ reqs).
+      iSplit.
+      { rewrite set_map_union_L set_map_singleton_L.
+        by iApply big_sepS_insert_2.
+      }
+      iSplit.
+      { iApply big_sepS_insert_2; [done | done]. }
+      iPureIntro.
+      apply set_Forall_union; last first.
+      { apply (set_Forall_impl _ _ _ Henc). intros m Hm. clear -Hm. set_solver. }
+      rewrite set_Forall_singleton.
+      exists req.
+      split; first set_solver.
+      done.
+    }
+    rewrite insert_delete_insert.
+    iMod "Hmask" as "_".
+    iMod ("HinvnetC" with "[$Hlistens $Hconnects $Hterminals]") as "_".
+    { iPureIntro.
+      rewrite dom_insert_L Himgaddrm.
+      apply (elem_of_map_img_2 (SA := gset chan)) in Haddrpeer.
+      set_solver.
+    }
+    iIntros "!> _".
+    wp_pures.
+    by iApply "HΦ".
+  Qed.
 
   Theorem wp_GroupCoordinator__SendPrepare
-    (gcoord : loc) (rid : u64) (tsW : u64) (rank : u64) gid γ :
+    (gcoord : loc) (rid : u64) (tsW : u64) addrm gid γ :
     let ts := uint.nat tsW in
+    rid ∈ dom addrm ->
     is_group_prepare_proposal γ gid ts 1%nat true -∗
-    is_gcoord gcoord gid γ -∗
+    is_gcoord_with_addrm gcoord gid addrm γ -∗
     {{{ True }}}
-      GroupCoordinator__SendPrepare #gcoord #rid #tsW #rank
+      GroupCoordinator__SendPrepare #gcoord #rid #tsW
     {{{ RET #(); True }}}.
   Proof.
-    (*@ func (gcoord *GroupCoordinator) SendPrepare(rid, ts, rank uint64) {     @*)
+    iIntros (ts Hrid) "#Hppsl #Hgcoord".
+    iIntros (Φ) "!> _ HΦ".
+    wp_rec.
+
+    (*@ func (gcoord *GroupCoordinator) SendPrepare(rid, ts uint64) {           @*)
+    (*@     data := message.EncodeTxnPrepareRequest(ts, 1)                      @*)
+    (*@     gcoord.Send(rid, data)                                              @*)
     (*@ }                                                                       @*)
-  Admitted.
+    wp_apply (wp_EncodeTxnPrepareRequest).
+    iIntros (dataP data) "(Hdata & %Hdataenc)".
+    iNamed "Hgcoord".
+    iNamed "Haddrm".
+    assert (is_Some (addrm !! rid)) as [addrpeer Haddrpeer].
+    { by apply elem_of_dom. }
+    wp_apply (wp_GroupCoordinator__Send with "[] Hdata"); first apply Haddrpeer.
+    { iFrame "# %". }
+    iInv "Hinvnet" as "> HinvnetO" "HinvnetC".
+    iApply ncfupd_mask_intro; first set_solver.
+    iIntros "Hmask".
+    iNamed "HinvnetO".
+    assert (is_Some (listens !! addrpeer)) as [ms Hms].
+    { rewrite -elem_of_dom -Himgaddrm elem_of_map_img. by eauto. }
+    iDestruct (big_sepM_delete with "Hlistens") as "[Hlst Hlistens]"; first apply Hms.
+    iNamed "Hlst".
+    iFrame "Hms".
+    iIntros (sent) "Hms".
+    destruct sent; last first.
+    { iDestruct (big_sepM_insert_2 _ _ addrpeer ms with "[Hms] Hlistens") as "Hlistens".
+      { iFrame "∗ # %". }
+      rewrite insert_delete; last apply Hms.
+      iMod "Hmask" as "_".
+      iMod ("HinvnetC" with "[$Hlistens $Hconnects $Hterminals]") as "_".
+      { done. }
+      iIntros "!> _".
+      wp_pures.
+      by iApply "HΦ".
+    }
+    iDestruct "Hms" as (trml) "[Hms #Htrml]".
+    set ms' := _ ∪ ms.
+    iDestruct (big_sepM_insert_2 _ _ addrpeer ms' with "[Hms] Hlistens") as "Hlistens".
+    { iFrame "Hms".
+      set req := PrepareReq _ _ in Hdataenc.
+      iExists ({[req]} ∪ reqs).
+      iSplit.
+      { rewrite set_map_union_L set_map_singleton_L.
+        by iApply big_sepS_insert_2.
+      }
+      iSplit.
+      { iApply big_sepS_insert_2; last done. by iFrame "Hppsl". }
+      iPureIntro.
+      apply set_Forall_union; last first.
+      { apply (set_Forall_impl _ _ _ Henc). intros m Hm. clear -Hm. set_solver. }
+      rewrite set_Forall_singleton.
+      exists req.
+      split; first set_solver.
+      done.
+    }
+    rewrite insert_delete_insert.
+    iMod "Hmask" as "_".
+    iMod ("HinvnetC" with "[$Hlistens $Hconnects $Hterminals]") as "_".
+    { iPureIntro.
+      rewrite dom_insert_L Himgaddrm.
+      apply (elem_of_map_img_2 (SA := gset chan)) in Haddrpeer.
+      set_solver.
+    }
+    iIntros "!> _".
+    wp_pures.
+    by iApply "HΦ".
+  Qed.
 
   Theorem wp_GroupCoordinator__SendUnprepare
-    (gcoord : loc) (rid : u64) (tsW : u64) (rank : u64) gid γ :
+    (gcoord : loc) (rid : u64) (tsW : u64) addrm gid γ :
     let ts := uint.nat tsW in
+    rid ∈ dom addrm ->
     is_group_prepare_proposal γ gid ts 1%nat false -∗
-    is_gcoord gcoord gid γ -∗
+    is_gcoord_with_addrm gcoord gid addrm γ -∗
     {{{ True }}}
-      GroupCoordinator__SendUnprepare #gcoord #rid #tsW #rank
+      GroupCoordinator__SendUnprepare #gcoord #rid #tsW
     {{{ RET #(); True }}}.
   Proof.
-    (*@ func (gcoord *GroupCoordinator) SendUnprepare(rid, ts, rank uint64) {   @*)
+    iIntros (ts Hrid) "#Hppsl #Hgcoord".
+    iIntros (Φ) "!> _ HΦ".
+    wp_rec.
+
+    (*@ func (gcoord *GroupCoordinator) SendUnprepare(rid, ts uint64) {         @*)
+    (*@     data := message.EncodeTxnUnprepareRequest(ts, 1)                    @*)
+    (*@     gcoord.Send(rid, data)                                              @*)
     (*@ }                                                                       @*)
-  Admitted.
+    wp_apply (wp_EncodeTxnUnprepareRequest).
+    iIntros (dataP data) "(Hdata & %Hdataenc)".
+    iNamed "Hgcoord".
+    iNamed "Haddrm".
+    assert (is_Some (addrm !! rid)) as [addrpeer Haddrpeer].
+    { by apply elem_of_dom. }
+    wp_apply (wp_GroupCoordinator__Send with "[] Hdata"); first apply Haddrpeer.
+    { iFrame "# %". }
+    iInv "Hinvnet" as "> HinvnetO" "HinvnetC".
+    iApply ncfupd_mask_intro; first set_solver.
+    iIntros "Hmask".
+    iNamed "HinvnetO".
+    assert (is_Some (listens !! addrpeer)) as [ms Hms].
+    { rewrite -elem_of_dom -Himgaddrm elem_of_map_img. by eauto. }
+    iDestruct (big_sepM_delete with "Hlistens") as "[Hlst Hlistens]"; first apply Hms.
+    iNamed "Hlst".
+    iFrame "Hms".
+    iIntros (sent) "Hms".
+    destruct sent; last first.
+    { iDestruct (big_sepM_insert_2 _ _ addrpeer ms with "[Hms] Hlistens") as "Hlistens".
+      { iFrame "∗ # %". }
+      rewrite insert_delete; last apply Hms.
+      iMod "Hmask" as "_".
+      iMod ("HinvnetC" with "[$Hlistens $Hconnects $Hterminals]") as "_".
+      { done. }
+      iIntros "!> _".
+      wp_pures.
+      by iApply "HΦ".
+    }
+    iDestruct "Hms" as (trml) "[Hms #Htrml]".
+    set ms' := _ ∪ ms.
+    iDestruct (big_sepM_insert_2 _ _ addrpeer ms' with "[Hms] Hlistens") as "Hlistens".
+    { iFrame "Hms".
+      set req := UnprepareReq _ _ in Hdataenc.
+      iExists ({[req]} ∪ reqs).
+      iSplit.
+      { rewrite set_map_union_L set_map_singleton_L.
+        by iApply big_sepS_insert_2.
+      }
+      iSplit.
+      { iApply big_sepS_insert_2; last done. by iFrame "Hppsl". }
+      iPureIntro.
+      apply set_Forall_union; last first.
+      { apply (set_Forall_impl _ _ _ Henc). intros m Hm. clear -Hm. set_solver. }
+      rewrite set_Forall_singleton.
+      exists req.
+      split; first set_solver.
+      done.
+    }
+    rewrite insert_delete_insert.
+    iMod "Hmask" as "_".
+    iMod ("HinvnetC" with "[$Hlistens $Hconnects $Hterminals]") as "_".
+    { iPureIntro.
+      rewrite dom_insert_L Himgaddrm.
+      apply (elem_of_map_img_2 (SA := gset chan)) in Haddrpeer.
+      set_solver.
+    }
+    iIntros "!> _".
+    wp_pures.
+    by iApply "HΦ".
+  Qed.
 
   Theorem wp_GroupCoordinator__SendQuery
-    (gcoord : loc) (rid : u64) (ts : u64) (rank : u64) gid γ :
-    is_gcoord gcoord gid γ -∗
+    (gcoord : loc) (rid : u64) (tsW : u64) addrm gid γ :
+    let ts := uint.nat tsW in
+    rid ∈ dom addrm ->
+    is_gcoord_with_addrm gcoord gid addrm γ -∗
     {{{ True }}}
-      GroupCoordinator__SendQuery #gcoord #rid #ts #rank
+      GroupCoordinator__SendQuery #gcoord #rid #tsW
     {{{ RET #(); True }}}.
   Proof.
-    (*@ func (gcoord *GroupCoordinator) SendQuery(rid, ts, rank uint64) {       @*)
+    iIntros (ts Hrid) "#Hgcoord".
+    iIntros (Φ) "!> _ HΦ".
+    wp_rec.
+
+    (*@ func (gcoord *GroupCoordinator) SendQuery(rid, ts uint64) {             @*)
+    (*@     data := message.EncodeTxnQueryRequest(ts, 1)                        @*)
+    (*@     gcoord.Send(rid, data)                                              @*)
     (*@ }                                                                       @*)
-  Admitted.
+    wp_apply (wp_EncodeTxnQueryRequest).
+    iIntros (dataP data) "(Hdata & %Hdataenc)".
+    iNamed "Hgcoord".
+    iNamed "Haddrm".
+    assert (is_Some (addrm !! rid)) as [addrpeer Haddrpeer].
+    { by apply elem_of_dom. }
+    wp_apply (wp_GroupCoordinator__Send with "[] Hdata"); first apply Haddrpeer.
+    { iFrame "# %". }
+    iInv "Hinvnet" as "> HinvnetO" "HinvnetC".
+    iApply ncfupd_mask_intro; first set_solver.
+    iIntros "Hmask".
+    iNamed "HinvnetO".
+    assert (is_Some (listens !! addrpeer)) as [ms Hms].
+    { rewrite -elem_of_dom -Himgaddrm elem_of_map_img. by eauto. }
+    iDestruct (big_sepM_delete with "Hlistens") as "[Hlst Hlistens]"; first apply Hms.
+    iNamed "Hlst".
+    iFrame "Hms".
+    iIntros (sent) "Hms".
+    destruct sent; last first.
+    { iDestruct (big_sepM_insert_2 _ _ addrpeer ms with "[Hms] Hlistens") as "Hlistens".
+      { iFrame "∗ # %". }
+      rewrite insert_delete; last apply Hms.
+      iMod "Hmask" as "_".
+      iMod ("HinvnetC" with "[$Hlistens $Hconnects $Hterminals]") as "_".
+      { done. }
+      iIntros "!> _".
+      wp_pures.
+      by iApply "HΦ".
+    }
+    iDestruct "Hms" as (trml) "[Hms #Htrml]".
+    set ms' := _ ∪ ms.
+    iDestruct (big_sepM_insert_2 _ _ addrpeer ms' with "[Hms] Hlistens") as "Hlistens".
+    { iFrame "Hms".
+      set req := QueryReq _ _ in Hdataenc.
+      iExists ({[req]} ∪ reqs).
+      iSplit.
+      { rewrite set_map_union_L set_map_singleton_L.
+        by iApply big_sepS_insert_2.
+      }
+      iSplit.
+      { by iApply big_sepS_insert_2. }
+      iPureIntro.
+      apply set_Forall_union; last first.
+      { apply (set_Forall_impl _ _ _ Henc). intros m Hm. clear -Hm. set_solver. }
+      rewrite set_Forall_singleton.
+      exists req.
+      split; first set_solver.
+      done.
+    }
+    rewrite insert_delete_insert.
+    iMod "Hmask" as "_".
+    iMod ("HinvnetC" with "[$Hlistens $Hconnects $Hterminals]") as "_".
+    { iPureIntro.
+      rewrite dom_insert_L Himgaddrm.
+      apply (elem_of_map_img_2 (SA := gset chan)) in Haddrpeer.
+      set_solver.
+    }
+    iIntros "!> _".
+    wp_pures.
+    by iApply "HΦ".
+  Qed.
 
   Theorem wp_GroupCoordinator__SendRefresh
-    (gcoord : loc) (rid : u64) (ts : u64) (rank : u64) gid γ :
-    is_gcoord gcoord gid γ -∗
+    (gcoord : loc) (rid : u64) (tsW : u64) addrm gid γ :
+    let ts := uint.nat tsW in
+    rid ∈ dom addrm ->
+    is_gcoord_with_addrm gcoord gid addrm γ -∗
     {{{ True }}}
-      GroupCoordinator__SendRefresh #gcoord #rid #ts #rank
+      GroupCoordinator__SendRefresh #gcoord #rid #tsW
     {{{ RET #(); True }}}.
   Proof.
-    (*@ func (gcoord *GroupCoordinator) SendRefresh(rid, ts, rank uint64) {     @*)
+    iIntros (ts Hrid) "#Hgcoord".
+    iIntros (Φ) "!> _ HΦ".
+    wp_rec.
+
+    (*@ func (gcoord *GroupCoordinator) SendRefresh(rid, ts uint64) {           @*)
+    (*@     data := message.EncodeTxnRefreshRequest(ts, 1)                      @*)
+    (*@     gcoord.Send(rid, data)                                              @*)
     (*@ }                                                                       @*)
-  Admitted.
+    wp_apply (wp_EncodeTxnRefreshRequest).
+    iIntros (dataP data) "(Hdata & %Hdataenc)".
+    iNamed "Hgcoord".
+    iNamed "Haddrm".
+    assert (is_Some (addrm !! rid)) as [addrpeer Haddrpeer].
+    { by apply elem_of_dom. }
+    wp_apply (wp_GroupCoordinator__Send with "[] Hdata"); first apply Haddrpeer.
+    { iFrame "# %". }
+    iInv "Hinvnet" as "> HinvnetO" "HinvnetC".
+    iApply ncfupd_mask_intro; first set_solver.
+    iIntros "Hmask".
+    iNamed "HinvnetO".
+    assert (is_Some (listens !! addrpeer)) as [ms Hms].
+    { rewrite -elem_of_dom -Himgaddrm elem_of_map_img. by eauto. }
+    iDestruct (big_sepM_delete with "Hlistens") as "[Hlst Hlistens]"; first apply Hms.
+    iNamed "Hlst".
+    iFrame "Hms".
+    iIntros (sent) "Hms".
+    destruct sent; last first.
+    { iDestruct (big_sepM_insert_2 _ _ addrpeer ms with "[Hms] Hlistens") as "Hlistens".
+      { iFrame "∗ # %". }
+      rewrite insert_delete; last apply Hms.
+      iMod "Hmask" as "_".
+      iMod ("HinvnetC" with "[$Hlistens $Hconnects $Hterminals]") as "_".
+      { done. }
+      iIntros "!> _".
+      wp_pures.
+      by iApply "HΦ".
+    }
+    iDestruct "Hms" as (trml) "[Hms #Htrml]".
+    set ms' := _ ∪ ms.
+    iDestruct (big_sepM_insert_2 _ _ addrpeer ms' with "[Hms] Hlistens") as "Hlistens".
+    { iFrame "Hms".
+      set req := RefreshReq _ _ in Hdataenc.
+      iExists ({[req]} ∪ reqs).
+      iSplit.
+      { rewrite set_map_union_L set_map_singleton_L.
+        by iApply big_sepS_insert_2.
+      }
+      iSplit.
+      { by iApply big_sepS_insert_2. }
+      iPureIntro.
+      apply set_Forall_union; last first.
+      { apply (set_Forall_impl _ _ _ Henc). intros m Hm. clear -Hm. set_solver. }
+      rewrite set_Forall_singleton.
+      exists req.
+      split; first set_solver.
+      done.
+    }
+    rewrite insert_delete_insert.
+    iMod "Hmask" as "_".
+    iMod ("HinvnetC" with "[$Hlistens $Hconnects $Hterminals]") as "_".
+    { iPureIntro.
+      rewrite dom_insert_L Himgaddrm.
+      apply (elem_of_map_img_2 (SA := gset chan)) in Haddrpeer.
+      set_solver.
+    }
+    iIntros "!> _".
+    wp_pures.
+    by iApply "HΦ".
+  Qed.
 
   Theorem wp_GroupCoordinator__SendCommit
-    (gcoord : loc) (rid : u64) (tsW : u64) (pwrsP : loc) q (pwrs : dbmap) gid γ :
+    (gcoord : loc) (rid : u64) (tsW : u64) (pwrsP : loc) q (pwrs : dbmap) addrm gid γ :
     let ts := uint.nat tsW in
+    rid ∈ dom addrm ->
     safe_commit γ gid ts pwrs -∗
-    is_gcoord gcoord gid γ -∗
+    is_gcoord_with_addrm gcoord gid addrm γ -∗
     {{{ own_map pwrsP q pwrs }}}
       GroupCoordinator__SendCommit #gcoord #rid #tsW #pwrsP
     {{{ RET #(); own_map pwrsP q pwrs }}}.
   Proof.
-    (*@ func (gcoord *GroupCoordinator) SendCommit(rid, ts uint64, pwrs tulip.KVMap) { @*)
-    (*@ }                                                                       @*)
-  Admitted.
+    iIntros (ts Hrid) "#Hsafecommit #Hgcoord".
+    iIntros (Φ) "!> Hpwrs HΦ".
+    wp_rec.
 
-  Theorem wp_GroupCoordinator__SendAbort (gcoord : loc) (rid : u64) (tsW : u64) gid γ :
+    (*@ func (gcoord *GroupCoordinator) SendCommit(rid, ts uint64, pwrs tulip.KVMap) { @*)
+    (*@     data := message.EncodeTxnCommitRequest(ts, pwrs)                    @*)
+    (*@     gcoord.Send(rid, data)                                              @*)
+    (*@ }                                                                       @*)
+    wp_apply (wp_EncodeTxnCommitRequest with "Hpwrs").
+    iIntros (dataP data) "(Hdata & Hpwrs & %Hdataenc)".
+    iNamed "Hgcoord".
+    iNamed "Haddrm".
+    assert (is_Some (addrm !! rid)) as [addrpeer Haddrpeer].
+    { by apply elem_of_dom. }
+    wp_apply (wp_GroupCoordinator__Send with "[] Hdata"); first apply Haddrpeer.
+    { iFrame "# %". }
+    iInv "Hinvnet" as "> HinvnetO" "HinvnetC".
+    iApply ncfupd_mask_intro; first set_solver.
+    iIntros "Hmask".
+    iNamed "HinvnetO".
+    assert (is_Some (listens !! addrpeer)) as [ms Hms].
+    { rewrite -elem_of_dom -Himgaddrm elem_of_map_img. by eauto. }
+    iDestruct (big_sepM_delete with "Hlistens") as "[Hlst Hlistens]"; first apply Hms.
+    iNamed "Hlst".
+    iFrame "Hms".
+    iIntros (sent) "Hms".
+    destruct sent; last first.
+    { iDestruct (big_sepM_insert_2 _ _ addrpeer ms with "[Hms] Hlistens") as "Hlistens".
+      { iFrame "∗ # %". }
+      rewrite insert_delete; last apply Hms.
+      iMod "Hmask" as "_".
+      iMod ("HinvnetC" with "[$Hlistens $Hconnects $Hterminals]") as "_".
+      { done. }
+      iIntros "!> _".
+      wp_pures.
+      by iApply "HΦ".
+    }
+    iDestruct "Hms" as (trml) "[Hms #Htrml]".
+    set ms' := _ ∪ ms.
+    iDestruct (big_sepM_insert_2 _ _ addrpeer ms' with "[Hms] Hlistens") as "Hlistens".
+    { iFrame "Hms".
+      set req := CommitReq _ _ in Hdataenc.
+      iExists ({[req]} ∪ reqs).
+      iSplit.
+      { rewrite set_map_union_L set_map_singleton_L.
+        by iApply big_sepS_insert_2.
+      }
+      iSplit.
+      { iApply big_sepS_insert_2; [done | done]. }
+      iPureIntro.
+      apply set_Forall_union; last first.
+      { apply (set_Forall_impl _ _ _ Henc). intros m Hm. clear -Hm. set_solver. }
+      rewrite set_Forall_singleton.
+      exists req.
+      split; first set_solver.
+      done.
+    }
+    rewrite insert_delete_insert.
+    iMod "Hmask" as "_".
+    iMod ("HinvnetC" with "[$Hlistens $Hconnects $Hterminals]") as "_".
+    { iPureIntro.
+      rewrite dom_insert_L Himgaddrm.
+      apply (elem_of_map_img_2 (SA := gset chan)) in Haddrpeer.
+      set_solver.
+    }
+    iIntros "!> _".
+    wp_pures.
+    by iApply "HΦ".
+  Qed.
+
+  Theorem wp_GroupCoordinator__SendAbort
+    (gcoord : loc) (rid : u64) (tsW : u64) addrm gid γ :
     let ts := uint.nat tsW in
+    rid ∈ dom addrm ->
     safe_abort γ ts -∗
-    is_gcoord gcoord gid γ -∗
+    is_gcoord_with_addrm gcoord gid addrm γ -∗
     {{{ True }}}
       GroupCoordinator__SendAbort #gcoord #rid #tsW
     {{{ RET #(); True }}}.
   Proof.
+    iIntros (ts Hrid) "#Hsafeabort #Hgcoord".
+    iIntros (Φ) "!> _ HΦ".
+    wp_rec.
+
     (*@ func (gcoord *GroupCoordinator) SendAbort(rid, ts uint64) {             @*)
+    (*@     data := message.EncodeTxnAbortRequest(ts)                           @*)
+    (*@     gcoord.Send(rid, data)                                              @*)
     (*@ }                                                                       @*)
-  Admitted.
+    wp_apply (wp_EncodeTxnAbortRequest).
+    iIntros (dataP data) "(Hdata & %Hdataenc)".
+    iNamed "Hgcoord".
+    iNamed "Haddrm".
+    assert (is_Some (addrm !! rid)) as [addrpeer Haddrpeer].
+    { by apply elem_of_dom. }
+    wp_apply (wp_GroupCoordinator__Send with "[] Hdata"); first apply Haddrpeer.
+    { iFrame "# %". }
+    iInv "Hinvnet" as "> HinvnetO" "HinvnetC".
+    iApply ncfupd_mask_intro; first set_solver.
+    iIntros "Hmask".
+    iNamed "HinvnetO".
+    assert (is_Some (listens !! addrpeer)) as [ms Hms].
+    { rewrite -elem_of_dom -Himgaddrm elem_of_map_img. by eauto. }
+    iDestruct (big_sepM_delete with "Hlistens") as "[Hlst Hlistens]"; first apply Hms.
+    iNamed "Hlst".
+    iFrame "Hms".
+    iIntros (sent) "Hms".
+    destruct sent; last first.
+    { iDestruct (big_sepM_insert_2 _ _ addrpeer ms with "[Hms] Hlistens") as "Hlistens".
+      { iFrame "∗ # %". }
+      rewrite insert_delete; last apply Hms.
+      iMod "Hmask" as "_".
+      iMod ("HinvnetC" with "[$Hlistens $Hconnects $Hterminals]") as "_".
+      { done. }
+      iIntros "!> _".
+      wp_pures.
+      by iApply "HΦ".
+    }
+    iDestruct "Hms" as (trml) "[Hms #Htrml]".
+    set ms' := _ ∪ ms.
+    iDestruct (big_sepM_insert_2 _ _ addrpeer ms' with "[Hms] Hlistens") as "Hlistens".
+    { iFrame "Hms".
+      set req := AbortReq _ in Hdataenc.
+      iExists ({[req]} ∪ reqs).
+      iSplit.
+      { rewrite set_map_union_L set_map_singleton_L.
+        by iApply big_sepS_insert_2.
+      }
+      iSplit.
+      { iApply big_sepS_insert_2; [done | done]. }
+      iPureIntro.
+      apply set_Forall_union; last first.
+      { apply (set_Forall_impl _ _ _ Henc). intros m Hm. clear -Hm. set_solver. }
+      rewrite set_Forall_singleton.
+      exists req.
+      split; first set_solver.
+      done.
+    }
+    rewrite insert_delete_insert.
+    iMod "Hmask" as "_".
+    iMod ("HinvnetC" with "[$Hlistens $Hconnects $Hterminals]") as "_".
+    { iPureIntro.
+      rewrite dom_insert_L Himgaddrm.
+      apply (elem_of_map_img_2 (SA := gset chan)) in Haddrpeer.
+      set_solver.
+    }
+    iIntros "!> _".
+    wp_pures.
+    by iApply "HΦ".
+  Qed.
 
 End program.
